fairness/locales_helpers.v
@@ -1,0 +1,34 @@
+From trillium.program_logic Require Import language adequacy.
+
+Section XX.
+  Context `{Countable (locale Λ)}.
+
+  Notation "'Tid'" := (locale Λ). 
+  
+  (* TODO: unify with existing locales_of_list_from_locale_from, 
+     remove restriction for Λ *)
+
+  Lemma locales_of_list_from_locale_from' tp0 tp1 ζ:
+    ζ ∈ locales_of_list_from tp0 tp1 (Λ := Λ) ->
+    is_Some (from_locale_from tp0 tp1 ζ).
+  Proof.
+    clear -tp0 tp1 ζ.
+    revert tp0; induction tp1 as [|e1 tp1 IH]; intros tp0.
+    { simpl. intros H. inversion H. }
+    simpl.
+    rewrite /locales_of_list_from /=. intros.
+    destruct (decide (locale_of tp0 e1 = ζ)); simplify_eq; first set_solver.
+    apply elem_of_cons in H as [?| ?]; [done| ].
+    set_solver.
+  Qed.
+
+  Lemma locale_step_from_locale_src `{EqDecision (expr Λ)} c1 c2 ζ:
+    locale_step c1 (Some ζ) c2 →
+    is_Some(from_locale c1.1 ζ).
+  Proof.
+    intros Hstep. inversion Hstep; simplify_eq=>//.
+    rewrite /from_locale. rewrite from_locale_from_Some; try done.
+    apply prefixes_from_spec; eauto.
+  Qed. 
+
+End XX.
